# Week 2 - Lab Sheet

```agda
{-# OPTIONS --without-K --safe #-}
module Pool.Lab.lab2 where

open import prelude hiding (if_then_else_;_||_)
```

## Part I: Booleans

### Section 1: Operations on Booleans

#### Exercise 1.1

We have already defined `if-then-else` like so:

```agda
if_then_else_ : {A : Type} ‚Üí Bool ‚Üí A ‚Üí A ‚Üí A
if true  then x else y = x
if false then x else y = y
```

But this requires our two branches to be of the same type A. Instead, we could
define `if-then-else` to have branches of different types, using the `Either`
datatype

```agda
data Either (A B : Type) : Type where
 left  : A ‚Üí Either A B
 right : B ‚Üí Either A B

if'_then_else_ : {A B : Type} ‚Üí Bool ‚Üí A ‚Üí B ‚Üí Either A B
if' true then x else y = left x
if' false then x else y = right y
```

**Define** this function.

#### Exercise 1.2

We can define the `_||_` function in (at least) two different ways, depending on
how much pattern-matching we wish to perform:

```agda
_||_ : Bool ‚Üí Bool ‚Üí Bool
true  || y = true
false || y = y

_||'_ : Bool ‚Üí Bool ‚Üí Bool
true  ||' true  = true
true  ||' false = true
false ||' true  = true
false ||' false = false
```

**Complete** the two holes for `_||_` and the four holes for `_||'_`.

The `_||_` operator is *associative*, meaning `a || (b || c) ‚â° (a || b) || c`.

We can prove this for both of our definitions:

```agda
||-assoc : (a b c : Bool)  ‚Üí a ||  (b ||  c) ‚â° (a ||  b) || c
||-assoc true b c = refl true
||-assoc false true c = refl true
||-assoc false false true = refl true
||-assoc false false false = refl false

||'-assoc : (a b c : Bool) ‚Üí a ||' (b ||' c) ‚â° (a ||' b) ||' c
||'-assoc true true true =   refl true
||'-assoc true true false =  refl true
||'-assoc true false true =  refl true
||'-assoc true false false = refl true
||'-assoc false true true =  refl true
||'-assoc false true false = refl true
||'-assoc false false true = refl true
||'-assoc false false false = refl false
```

**Complete** both of these proofs.
(Hint: Because `||` was defined by pattern matching on the first argument, it
may be helpful to use the same strategy.)

Which of these did you prefer proving, and why?

#### Exercise 1.3

**Complete** the proof that Boolean disjunction is commutative:

```agda
||-is-commutative : (a b : Bool) ‚Üí a || b ‚â° b || a
||-is-commutative true true = refl true
||-is-commutative true false = refl true
||-is-commutative false true = refl true
||-is-commutative false false = refl false
```

#### Exercise 1.4

**Complete** the proof that `false` is the left unit element of `||`:

```agda
false-left-unit-for-|| : (b : Bool) ‚Üí false || b ‚â° b
false-left-unit-for-|| b = refl b
```

**Complete** the proof that `false` is the right unit element of `||`:

```agda
false-right-unit-for-|| : (b : Bool) ‚Üí b || false ‚â° b
false-right-unit-for-|| true = refl true
false-right-unit-for-|| false = refl false
```

#### Exercise 1.5

Now prove the analogous properties for `&&`.

**Complete** the proof that Boolean conjunction is associative:

```agda
&&-is-associative : (a b c : Bool) ‚Üí a && (b && c) ‚â° (a && b) && c
&&-is-associative a b c = {!!}
```

**Complete** the proof that Boolean conjunction is commutative:

```agda
&&-is-commutative : (a b : Bool) ‚Üí a && b ‚â° b && a
&&-is-commutative a b = {!!}
```

**Complete** the proof that that `true` is the left unit element of `&&`:

```agda
true-left-unit-for-&& : (b : Bool) ‚Üí true && b ‚â° b
true-left-unit-for-&& b = {!!}
```

**Complete** the proof that that `true` is the right unit element of `&&`:

```agda
true-right-unit-for-&& : (b : Bool) ‚Üí b && true ‚â° b
true-right-unit-for-&& b = {!!}
```

#### Exercise 1.6

An important algebraic property between two operators is *distributivity*. For
example, multiplication distributes over addition since `x * (y + z) = (x * y) +
(x * z)` for every `x, y, z ‚àà ‚Ñï`. The same is the case for the Boolean
conjunction and disjunction operators we have defined.

**Complete** the proof that Boolean conjunction distributes over Boolean
disjunction:

```agda
&&-distributes-over-|| : (a b c : Bool) ‚Üí a && (b || c) ‚â° (a && b) || (a && c)
&&-distributes-over-|| a b c = {!!}
```

```agda
||-distributes-over-&& : (a b c : Bool) ‚Üí a || (b && c) ‚â° (a || b) && (a || c)
||-distributes-over-&& a b c = {!!}
```


### Section 2: Identity type and `Bool`

With these exercises, you will practise with the identity type and `Bool`.

#### Exercise 2.1

Recall how we defined `_‚â£_` for [natural
numbers](../introduction.lagda.md#the-empty-type-and-the-unit-type). We could do
the same for the Booleans.

```agda
_‚â£_ : Bool ‚Üí Bool ‚Üí Type
true ‚â£ true = ùüô
true ‚â£ false = ùüò
false ‚â£ true = ùüò
false ‚â£ false = ùüô
```

**Define** this function.

Tip: you can type `‚â£` as `\===`.

#### Exercise 2.2

We can also define a Boolean-valued equality function.

```agda
_==_ : Bool ‚Üí Bool ‚Üí Bool
true == y = y
false == y = not y
```

**Define** this function.

#### Exercise 2.3

Now we write a conversion function from `x ‚â° y` to `x ‚â£ y`, just like the
function `back` in
[introduction](../introduction.lagda.md#the-identity-type-former-__).

```agda
‚â£-refl : ‚àÄ x ‚Üí x ‚â£ x
‚â£-refl true = ‚ãÜ
‚â£-refl false = ‚ãÜ

‚â°-to-‚â£ : (x y : Bool) ‚Üí x ‚â° y ‚Üí x ‚â£ y
‚â°-to-‚â£ = ‚â°-nondep-elim _‚â£_ ‚â£-refl 
```

**Complete** this function.

#### Exercise 2.4

The following helper function makes some functions nicer to read.

```agda
is-true : Bool ‚Üí Type
is-true b = b ‚â° true
```

Now we can consider another conversion function.

```agda
‚â£-to-== : (x y : Bool) ‚Üí x ‚â£ y ‚Üí is-true (x == y)
‚â£-to-== true true _   = refl true
‚â£-to-== false false _ = refl true
```

**Define** this function.

#### Exercise 2.5

And similarly, we have

```agda
==-to-‚â° : (x y : Bool) ‚Üí is-true (x == y) ‚Üí x ‚â° y
==-to-‚â° true true _   = refl true
==-to-‚â° false false _ = refl false
```

**Define** this function.

#### Exercise 2.6

Finally, we can use the above functions to define the three remaining
implications

```agda
‚â°-to-== : (x y : Bool) ‚Üí x ‚â° y ‚Üí is-true (x == y)
‚â°-to-== x y = (‚â£-to-== x y) ‚àò (‚â°-to-‚â£ x y)

‚â£-to-‚â° : (x y : Bool) ‚Üí x ‚â£ y ‚Üí x ‚â° y
‚â£-to-‚â° x y = (==-to-‚â° x y) ‚àò (‚â£-to-== x y)

==-to-‚â£ : (x y : Bool) ‚Üí is-true (x == y) ‚Üí x ‚â£ y
==-to-‚â£ x y = (‚â°-to-‚â£ x y) ‚àò (==-to-‚â° x y)
```

**Complete** these functions.


## Part II: Natural numbers

### Section 1: Some functions on natural numbers

#### Exercise 1.1

**Complete** the proof of the fact that `(suc x) + y ‚â° suc (x + y)`

```agda
+-suc-on-left : (x y : ‚Ñï) ‚Üí (suc x) + y ‚â° suc (x + y)
+-suc-on-left x y = {!!}
```

#### Exercise 1.2

We can define `max` operation on natural numbers as follows:

```agda
max : ‚Ñï ‚Üí ‚Ñï ‚Üí ‚Ñï
max zero    n       = n
max (suc m) zero    = suc m
max (suc m) (suc n) = suc (max m n)
```

**Define** the function `min` analogously:

```agda
min : ‚Ñï ‚Üí ‚Ñï ‚Üí ‚Ñï
min zero    n       = zero
min (suc m) zero    = zero
min (suc m) (suc n) = suc (min m n)

```

### Section 2: Natural numbers and proofs using induction

The function `+-0-on-right` expresses the fact that `0` is a right unit of the
operation `_+_`. Notice how we use an inductive hypothesis (the recursive call)
in the proof. (Spelling this out, `IH` tells us that `x + 0 ‚â° x`, so that `ap
suc IH` witnesses that `suc (x + 0) ‚â° suc x`.)

```agda
+-0-on-right : (x : ‚Ñï) ‚Üí x + 0 ‚â° x
+-0-on-right zero    = refl zero
+-0-on-right (suc x) = ap suc IH
 where
  IH : x + 0 ‚â° x -- IH is short for induction hypothesis
  IH = +-0-on-right x
```

Using similar induction hypotheses, try to complete the following exercises.


#### Exercise 2.1

**Complete** the proof:

```agda
+-suc-on-right : (x y : ‚Ñï) ‚Üí x + suc y ‚â° suc (x + y)
+-suc-on-right zero    y = refl (suc y)
+-suc-on-right (suc x) y = ap suc (+-suc-on-right x y)
```

#### Exercise 2.2

In algebra, an operator `_*_` is called idempotent iff `x * x = x` for every
`x`. `max` is an example of an idempotent operator:

**Complete** the hole to prove that `max` is idempotent:

```agda
max-idempotent : (x : ‚Ñï) ‚Üí max x x ‚â° x
max-idempotent zero    = refl zero
max-idempotent (suc x) = ap suc (max-idempotent x)
```

#### Exercise 2.3

**Complete** the hole by constructing a proof of the fact that `max` is a
commutative operator:

```agda
max-commutative : (x y : ‚Ñï) ‚Üí max x y ‚â° max y x
max-commutative zero    zero    = refl zero
max-commutative zero    (suc y) = refl (suc y)
max-commutative (suc x) zero    = refl (suc x)
max-commutative (suc x) (suc y) = ap suc (max-commutative x y)
```

#### Exercise 2.4

Now recall that we defined `min` in Exercise 1.2. Similarly, we can show that
`min` is idempotent and commutative too.

**Complete** the proof that `min` is idempotent:

```agda
min-idempotent : (x : ‚Ñï) ‚Üí min x x ‚â° x
min-idempotent zero    = refl zero
min-idempotent (suc x) = ap suc (min-idempotent x)
```

#### Exercise 2.5

**Complete** the proof that `min` is commutative:

```agda
min-commutative : (x y : ‚Ñï) ‚Üí min x y ‚â° min y x
min-commutative zero    zero    = refl zero
min-commutative zero    (suc y) = refl zero
min-commutative (suc x) zero    = refl zero
min-commutative (suc x) (suc y) = ap suc (min-commutative x y)
```
